WIP on completeness for existential HL.

theories/EHoare.v
@@ -39,9 +39,9 @@ Section EHoare.
   | EH_Spec : forall Q y f xs,
       Sigma |- {[fun st =>
             (Sigma f).(pre) (aseval st xs) /\
-            exists v, (Sigma f).(post) v (aseval st xs) /\
-                      forall v, (Sigma f).(post) v (aseval st xs) ->
-                 Q[y |-> v] st]} y :::= f $ xs {[Q]}#
+            (exists v, (Sigma f).(post) v (aseval st xs)) /\
+            forall v, (Sigma f).(post) v (aseval st xs) ->
+                      Q[y |-> v] st]} y :::= f $ xs {[Q]}#
 
   where "Sigma |- {[ P ]}  c  {[ Q ]}#" := (ehoare_proof Sigma P c Q) : hoare_spec_scope.
 
@@ -101,7 +101,7 @@ Section EHoare.
     - (* :::= *)
       destruct_conjs.
       repeat econstructor; eauto.
-      eapply H2; eauto.
+      eapply H1; eauto.
   Qed.
 
   Definition ewp (Sigma : Env) (c:com) (Q:Assertion) : Assertion :=
@@ -169,94 +169,8 @@ Section EHoare.
       auto.
   Qed.
 
-  (* Pretty sure this is the completeness statement we want. *)
-  Theorem ehoare_proof_complete Sigs Sigma : forall P c Q,
-      (forall funDefs,
-          productive_Env {| funSigs := Sigs; funSpecs := Sigma; funDefs := funDefs |}
-          -> {| funSigs := Sigs; funSpecs := Sigma; funDefs := funDefs |} |= {[P]} c {[Q]}#)
-      -> Sigma |- {[P]} c {[Q]}#.
-  Proof.
-    unfold ehoare_triple.
-    intros P c. revert dependent P.
-    induction c; intros P Q HT.
-    - (* SKIP *)
-      specialize (HT _ (productive_empty _ _)).
-      eapply EH_Consequence; eauto with hoare.
-      intros. edestruct HT as [? [exe ?]]; eauto.
-      inversion exe; subst. eauto.
-    - (* ::= *)
-      specialize (HT _ (productive_empty _ _)).
-      eapply EH_Consequence; eauto with hoare.
-      intros. edestruct HT as [? [exe ?]]; eauto.
-      inversion exe; subst. eauto.
-    - (* :::= *)
-      eapply EH_Consequence; eauto with hoare.
-      simpl. intros.
-      generalize (HT _ (productive_empty _ _)) as HT'; intros.
-      edestruct HT' as [? [exe ?]]; eauto; clear HT'.
-      admit.
-      (*inversion exe; subst.
-      + firstorder; eauto.
-        eexists _; split; eauto.
-        intros.
-        assert (productive_Env {| funSigs := Sigs;
-                                  funSpecs := Sigma;
-                                  funDefs := update empty f {| funArgs := nil;
-                                                               funBody := SKIP;
-                                                               funRet := v |} |}).
-        { unfold productive_Env; simpl; intros.
-          eapply update_inv in H2; intuition; subst.
-          - unfold productive_funDef; intros.
-            simpl.
-            eassert (Productive
-                                 {|
-                                 funSigs := Sigs;
-                                 funSpecs := Sigma;
-                                 funDefs := f0 |-> {| funArgs := nil; funBody := SKIP; funRet := v |} |} SKIP
-                                 (build_total_map nil args0 0) _).
-            econstructor.
-            simpl; eexists _, H3; eauto.
-            intros.
-      admit.
-          - compute in H5; discriminate.
-        } 
-        admit.
-      + *)
-    - (* ;; *)
-      apply EH_Seq with (@ewp {| funSigs := Sigs; funSpecs := Sigma; funDefs := empty |} c2 Q); eauto. apply IHc1.
-      intros.
-  (* edestruct HT as [? [exe ?]]; eauto.
-      inversion exe; subst. repeat econstructor; eauto.
-
--     
-      eapply IHc1.
-    - (* IFB *)
-      apply EH_If.
-      + apply IHc1. intros. destruct_conjs.
-        edestruct HT as [? [exe ?]]; eauto.
-        inversion exe; subst; firstorder with hoare.
-      + apply IHc2. intros. destruct_conjs.
-        edestruct HT as [? [exe ?]]; eauto.
-        inversion exe; subst; firstorder with hoare.
-    - (* WHILE *)
-      eapply EH_Consequence
-        (* These two conjunction components are actually equivalent. See ewp_loop_measureR *)
-        with (P':=fun st => ewp _ (WHILE b DO c END) Q st /\ exists n, loop_measureR _ b c Q n st).
-      + apply EH_While.
-        intros. apply IHc. intros st [Hwp [Hb Hm]].
-        edestruct (@loop_measureR_smallest_ex {| funSigs := Sigs; funSpecs := Sigma; funDefs := empty |}) as [st' [exe [HQ H]]]; eauto.
-        remember (WHILE b DO c END)%imp eqn:Heq.
-        destruct exe; inversion Heq; subst; clear Heq. exfalso. congruence.
-        unfold loop_measureR in *. destruct_conjs. subst. simpl in H.
-        exists st'. firstorder eauto.
-        eexists exe1; firstorder eauto.
-        eexists _; split.
-        eexists _, exe2; firstorder eauto.
-        subst; eauto.
-      + setoid_rewrite <- ewp_loop_measureR. firstorder eauto.
-      + simpl. intros ? [H ?]. destruct H as [? [exe ?]].
-        inversion exe; subst; eauto. exfalso. eauto. *)
-  Admitted.
+  Local Hint Constructors ceval.
+  Local Hint Constructors AppearsIn.
 
   Hint Constructors Productive : hoare.
 
@@ -296,33 +210,12 @@ Section EHoare.
         inversion H2; subst; intuition.
         eapply bassn_eval_false; eauto.
     - eapply Productive_Weaken; eauto.
-    - destruct H0 as [? [n [? ?] ] ].
+    - destruct H0 as [? [ [n ?] ?] ] .
       eapply Productive_Weaken; eauto.
       + eapply Productive_CallSpec; firstorder eauto.
       + unfold Included, In; intros.
         destruct H3 as [n' [? ?] ]; subst.
         eapply H2; eauto.
-  Qed.
-
-  (* The Productive predicate and the existential hoare rules should
-  be equivalent. This proof will let us prove the soundness of vc
-  generation with respect to the hoare rules. *)
-
-  Theorem produces_ehoare_proof {Sigma : Env}
-    : forall (P Q : Assertion) c,
-      productive_Env Sigma ->
-      (forall st,
-        P st ->
-        Productive {| funSigs := @funSigs Sigma;
-                      funSpecs := @funSpecs Sigma;
-                      funDefs := empty |} c st Q) ->
-        funSpecs |- {[P]} c {[Q]}#.
-  Proof.
-    intros; eapply ehoare_proof_complete.
-    intros.
-    unfold ehoare_triple; intros.
-    eapply productive_com_produces.
-    eapply productive_Env_produces; eauto.
   Qed.
 
   Theorem ehoare_proof_link {Sigma : Env}
@@ -336,6 +229,431 @@ Section EHoare.
     eapply productive_Env_produces; eauto.
     eapply ehoare_proof_produces; eauto.
   Qed.
+
+  (* WIP on completeness proofs. *)
+
+  (*Lemma ex_fully_permissive_funDef
+    : forall Sigs Sigma P Q f x args,
+      (forall funDefs,
+          productive_Env {| funSigs := Sigs; funSpecs := Sigma; funDefs := funDefs |}
+          -> {| funSigs := Sigs; funSpecs := Sigma; funDefs := funDefs |} |= {[P]} x :::= f $ args {[Q]}#) ->
+      exists fd : funDef,
+        ~ AppearsIn f (funBody fd) /\
+        productive_funDef {| funSigs := Sigs; funSpecs := Sigma; funDefs := empty |} (Sigma f) fd.
+  Proof.
+  Admitted. *)
+
+  (* Pretty sure this is the completeness statement we want. *)
+  (*Theorem ehoare_proof_complete Sigs Sigma : forall P c Q,
+      (forall funDefs,
+          productive_Env {| funSigs := Sigs; funSpecs := Sigma; funDefs := funDefs |}
+          -> {| funSigs := Sigs; funSpecs := Sigma; funDefs := funDefs |} |= {[P]} c {[Q]}#)
+      -> Sigma |- {[P]} c {[Q]}#.
+  Proof.
+    intros P c. revert dependent P.
+    induction c; intros P Q HT.
+    - (* SKIP *)
+      specialize (HT _ (productive_empty _ _)).
+      eapply EH_Consequence; eauto with hoare.
+      intros. edestruct HT as [? [exe ?]]; eauto.
+      inversion exe; subst. eauto.
+    - (* ::= *)
+      specialize (HT _ (productive_empty _ _)).
+      eapply EH_Consequence; eauto with hoare.
+      intros. edestruct HT as [? [exe ?]]; eauto.
+      inversion exe; subst. eauto.
+    - (* :::= *)
+      eapply EH_Consequence; eauto with hoare.
+      simpl. intros.
+      generalize (HT _ (productive_empty _ _)) as HT'; intros.
+      edestruct HT' as [? [exe ?]]; eauto; clear HT'.
+      inversion exe; subst.
+      + firstorder; eauto.
+        destruct (ex_fully_permissive_funDef _ _ _ _ _ _ _ HT) as [? [? ?] ].
+        assert (productive_Env {| funSigs := Sigs;
+                                  funSpecs := Sigma;
+                                  funDefs := update empty f x0 |}).
+        { eapply productive_Env_Extend with
+              (Sigma := {| funSigs := Sigs;
+                           funSpecs := Sigma;
+                           funDefs := empty |}); eauto using productive_empty.
+          simpl; intros; discriminate. }
+        generalize (HT _ H5) as HT'; intros.
+        edestruct HT' as [? [exe' ?] ]; eauto.
+        inversion exe'; subst.
+        * simpl in H12; unfold update in H12; rewrite t_update_eq in H12; congruence.
+        * apply update_inv in H14; intuition; subst.
+          simpl in H6.
+          eapply H6.
+      + compute in H6; discriminate.
+    - (* ;; *)
+      (*apply EH_Seq with (@ewp {| funSigs := Sigs; funSpecs := Sigma; funDefs := empty |} c2 Q); eauto. apply IHc1.
+      intros.
+      destruct (HT _ H _ H0) as [? [exe ?] ].
+      inversion exe; subst. repeat econstructor; eauto.
+
+
+-
+      eapply IHc1.
+    - (* IFB *)
+      apply EH_If.
+      + apply IHc1. intros. destruct_conjs.
+        edestruct HT as [? [exe ?]]; eauto.
+        inversion exe; subst; firstorder with hoare.
+      + apply IHc2. intros. destruct_conjs.
+        edestruct HT as [? [exe ?]]; eauto.
+        inversion exe; subst; firstorder with hoare.
+    - (* WHILE *)
+      eapply EH_Consequence
+        (* These two conjunction components are actually equivalent. See ewp_loop_measureR *)
+        with (P':=fun st => ewp _ (WHILE b DO c END) Q st /\ exists n, loop_measureR _ b c Q n st).
+      + apply EH_While.
+        intros. apply IHc. intros st [Hwp [Hb Hm]].
+        edestruct (@loop_measureR_smallest_ex {| funSigs := Sigs; funSpecs := Sigma; funDefs := empty |}) as [st' [exe [HQ H]]]; eauto.
+        remember (WHILE b DO c END)%imp eqn:Heq.
+        destruct exe; inversion Heq; subst; clear Heq. exfalso. congruence.
+        unfold loop_measureR in *. destruct_conjs. subst. simpl in H.
+        exists st'. firstorder eauto.
+        eexists exe1; firstorder eauto.
+        eexists _; split.
+        eexists _, exe2; firstorder eauto.
+        subst; eauto.
+      + setoid_rewrite <- ewp_loop_measureR. firstorder eauto.
+      + simpl. intros ? [H ?]. destruct H as [? [exe ?]].
+        inversion exe; subst; eauto. exfalso. eauto. *)
+  Admitted. *)
+
+  Inductive Productive_Bound {Sigma : Env}
+    : forall {st c Q}
+              (prod : Productive Sigma c st Q), nat -> Prop :=
+  | Bound_Skip :
+      forall st n, Productive_Bound (Productive_Skip Sigma st) n
+  | Bound_Ass :
+      forall st x a n, Productive_Bound (Productive_Ass Sigma st x a) n
+  | Bound_Seq : forall c1 c2 st Q Q' H H' n,
+      Productive_Bound (Productive_Seq Sigma c1 c2 st Q Q' H H') n
+  | Bound_IfTrue : forall st Q b c1 c2 H H' n,
+      Productive_Bound (Productive_IfTrue Sigma st Q b c1 c2 H H') n
+  | Bound_IfFalse : forall st Q b c1 c2 H H' n,
+      Productive_Bound (Productive_IfFalse Sigma st Q b c1 c2 H H') n
+  | Bound_WhileFalse : forall b st c H n,
+      Productive_Bound (Productive_WhileFalse Sigma b st c H) n
+  | Bound_WhileTrue : forall st b c (Q Q' : state -> Prop) beval_true prod_c prod_loop n,
+      (forall st' (Q_st' : Q st'), Productive_Bound (prod_loop _ Q_st') n) ->
+      Productive_Bound (Productive_WhileTrue Sigma st b c Q Q' beval_true prod_c prod_loop) (S n)
+  | Bound_CallDef :
+      forall st Q args x f fd H H' n,
+        Productive_Bound (Productive_CallDef Sigma st Q args x f fd H H') n
+  | Bound_CallSpec : forall st args x f n H H' H'' n',
+      Productive_Bound (Productive_CallSpec Sigma st args x f n H H' H'') n'
+  | Bound_Weaken : forall st c Q Q' H H' n,
+      Productive_Bound H n -> 
+      Productive_Bound (Productive_Weaken Sigma st c Q Q' H H') n.
+
+  Definition ewp' (Sigma : Env) (c:com) (Q:Assertion) : Assertion :=
+    fun st => Productive Sigma c st Q.
+
+  Definition loop_measureR' (Sigma : Env) b c Q n st : Prop :=
+    forall (prod : Productive Sigma (WHILE b DO c END) st Q),
+      Productive_Bound prod n.
+
+  Fixpoint Productive_ind'
+           (Sigma : Env) (P : forall (c : com) (st : state) (Q : Ensemble state),
+                             Productive Sigma c st Q -> Prop)
+           (f : forall st : state, P SKIP%imp st (Singleton state st) (Productive_Skip Sigma st))
+           (f0 : forall (st : state) (x : String.string) (a : aexp),
+               P (x ::= a)%imp st (Singleton (String.string -> nat) (x !-> aeval st a; st))
+                 (Productive_Ass Sigma st x a))
+           (f1 : forall (c1 c2 : com) (st : state) (Q Q' : Ensemble state)
+                        (H : Productive Sigma c1 st Q)
+                        (IH : P c1 st Q H) 
+                        (H' : forall st' : state, Q st' -> Productive Sigma c2 st' Q'),
+               (forall (st' : state) (Q_st' : Q st'), P c2 st' Q' (H' _ Q_st')) ->
+               P (c1;; c2)%imp st Q' (Productive_Seq Sigma c1 c2 st Q Q' H H'))
+           (f2 : forall (st : state) (Q : Ensemble state) (b : bexp) (c1 c2 : com)
+                        (H : beval st b = true)
+                        (H' : Productive Sigma c1 st Q)
+                        (IH : P c1 st Q H'),
+               P (TEST b THEN c1 ELSE c2 FI)%imp st Q (Productive_IfTrue Sigma st Q b c1 c2 H H'))
+           (f3 : forall (st : state) (b : bexp) (c1 c2 : com) (Q : Ensemble state)
+                        (H : beval st b = false)
+                        (H' : Productive Sigma c2 st Q)
+                        (IH : P c2 st Q H'),
+               P (TEST b THEN c1 ELSE c2 FI)%imp st Q (Productive_IfFalse Sigma st b c1 c2 Q H H'))
+           (f4 : forall (b : bexp) (st : state) (c : com)
+                        (H : beval st b = false),
+               P (WHILE b DO c END)%imp st (Singleton state st) (Productive_WhileFalse Sigma b st c H))
+           (f5 : forall (st : state) (b : bexp) (c : com) (Q Q' : Ensemble state)
+                        (H : beval st b = true)
+                        (H' : Productive Sigma c st Q)
+                        (IH : P c st Q H')
+                        (H'' : forall st' : state, Q st' -> Productive Sigma (WHILE b DO c END) st' Q')
+                        (IH2 : forall (st' : state) (Q_st' : Q st'), P (WHILE b DO c END)%imp st' Q' (H'' _ Q_st')),
+               P (WHILE b DO c END)%imp st Q' (Productive_WhileTrue Sigma st b c Q Q' H H' H''))
+           (f6 : forall (st : state) (Q : Ensemble state) (args : list aexp) (x f6 : String.string) (fd : funDef)
+                        (H : funDefs f6 = Some fd)
+                        (H' : Productive Sigma (funBody fd) (build_total_map (funArgs fd) (aseval st args) 0) Q)
+                        (IH : P (funBody fd) (build_total_map (funArgs fd) (aseval st args) 0) Q H'),
+               P (x :::= f6 $ args)%imp st
+                 (fun st' : state => exists st'' : state, Q st'' /\ st' = (x !-> aeval st'' (funRet fd); st))
+                 (Productive_CallDef Sigma st Q args x f6 fd H H'))
+           (f7 : forall (st : state) (args : list aexp) (x f7 : String.string) (n : nat)
+                        (H : funDefs f7 = None)
+                        (H' : pre (funSpecs f7) (aseval st args))
+                        (H'' : post (funSpecs f7) n (aseval st args)),
+               P (x :::= f7 $ args)%imp st
+                 (fun st' : state => exists n0 : nat, post (funSpecs f7) n0 (aseval st args) /\ st' = (x !-> n0; st))
+                 (Productive_CallSpec Sigma st args x f7 n H H' H''))
+           (f8 : forall (st : state) (c : com) (Q Q' : Ensemble state)
+                        (H : Productive Sigma c st Q)
+                        (IH : P c st Q H)
+                        (H' : Included state Q Q'),
+               P c st Q' (Productive_Weaken Sigma st c Q Q' H H'))    
+           (c : com) (s : state) (e : Ensemble state) (p : Productive Sigma c s e) {struct p} : 
+    P c s e p.
+  Proof.
+    destruct p; eauto.
+    - eapply f1.
+      eapply Productive_ind'; eauto.
+      intros; eapply Productive_ind'; eauto.
+    - eapply f2.
+      eapply Productive_ind'; eauto.
+    - eapply f3.
+      eapply Productive_ind'; eauto.
+    - eapply f5.
+      eapply Productive_ind'; eauto.
+      intros; eapply Productive_ind'; eauto.
+    - eapply f6.
+      eapply Productive_ind'; eauto.
+    - eapply f8.
+      eapply Productive_ind'; eauto.
+  Defined.
+        
+  Lemma ewp'_loop_measureR' (Sigma : Env) b c Q st
+    : ewp' Sigma (WHILE b DO c END) Q st -> exists n, loop_measureR' Sigma b c Q n st.
+  Proof.
+    unfold ewp', loop_measureR'; intros.
+    remember (CWhile b c).
+    revert dependent b; revert c.
+    pattern c0, st, Q, H.
+    eapply Productive_ind'; intros;
+    try solve [match goal with
+                   |- context [Productive _ ?c _ _] =>
+                   exists 0; intros;
+                   remember c; destruct prod; try discriminate; injections;
+                   try congruence; try econstructor
+                 end].
+    - injections.
+      match goal with
+        |- context [Productive _ ?c _ ?st'] =>
+                   exists 0; intros;
+                   remember c; remember st'
+                 end.
+      revert Heqc.
+      revert dependent b0; revert c1; clear Heqe.
+      pattern c, st0, e, prod.
+      eapply Productive_ind'; intros; try discriminate; injections;
+        try congruence; econstructor; eauto.
+    - injections.
+      admit.
+    - 
+      
+      (*with (P := (fun (c : com) (s : state) (e0 : Ensemble state) (p : Productive Sigma c s e0) =>
+   e0 = Singleton state s ->
+   forall (c1 : com) (b : bexp), beval s b = false -> c = (WHILE b DO c1 END)%imp -> Productive_Bound p 0))
+      remember ((Singleton state st))
+      econstructor.
+      econstructor.
+      
+      subst; injections.
+      
+      injections; exists 0.
+      intros.
+      2: { eexists 0; intros.
+
+
+    match goal with
+      |- context [Productive _ ?c _ _] =>
+      exists 0; intros;
+        remember c
+    end.
+    induction prod. try discriminate; injections;
+          try congruence; try econstructor
+
+
+
+    Focus 2.
+    destruct IHProductive.
+
+    match goal with
+      |- context [Productive _ ?c _ _] =>
+      exists 0; intros;
+        remember c; destruct prod; try discriminate; injections;
+          try congruence; try econstructor
+    end.
+    eapply Bound_CallSpec.
+
+    econstructor.
+      exists 0; intros;
+      remember CSkip; destruct prod; try discriminate; econstructor.
+    - exists 0; intros;
+      remember CSkip; destruct prod; try discriminate; econstructor.
+    - intros H.
+      eapply productive_com_produces in H.
+      destruct H as [st' [exe HQ]].
+      exists (loop_size exe). firstorder eauto.
+    - firstorder.
+  Qed. *)
+  Admitted.
+  (*Lemma loop_measureR_smallest_ex (Sigma : Env) b c Q st :
+    (exists st' (exe : Sigma |- st =[ WHILE b DO c END ]=> st'), Q st') ->
+    exists st' (exe : Sigma |- st =[ WHILE b DO c END ]=> st'),
+      Q st' /\
+      (forall st'' (exe' : Sigma |- st =[ WHILE b DO c END ]=> st''),
+          Q st'' -> loop_size exe <= loop_size exe').
+  Proof.
+    intros.
+    edestruct (nonempty_smallest_ex
+                 (fun m => exists st' (exe : Sigma |- st =[ WHILE b DO c END ]=> st'),
+                      Q st' /\ loop_size exe = m)).
+    - firstorder eauto.
+    - destruct_conjs. subst. repeat econstructor; eauto.
+      Grab Existential Variables.
+      auto.
+  Qed. *)
+
+  (*Fixpoint productive_bound {Sigma : Env} {st c Q}
+           (prod : Productive Sigma c st Q) {struct prod} : Prop :=
+    match prod return Prop with
+    | Productive_WhileTrue _ _ _ Q' _ _ _ _ exew => True
+    | _ => True
+    end.
+
+  (Sigma : Env) b c Q n st : Prop :=
+    (exists st' (exe : Sigma |- st =[ WHILE b DO c END ]=> st'),
+        Q st' /\
+        n = loop_size exe).
+
+  Lemma nonempty_smallest_ex (P : nat -> Prop) :
+    (exists n, P n) ->
+    exists n, P n /\ (forall n', P n' -> n <= n').
+  Proof.
+    intros [n H]. induction n using (well_founded_ind lt_wf).
+    destruct (classic (exists y, y < n /\ P y)).
+    - firstorder.
+    - exists n. intuition. apply Nat.nlt_ge. eauto.
+  Qed.
+
+  Lemma loop_measureR_smallest_ex (Sigma : Env) b c Q st :
+    (exists st' (exe : Sigma |- st =[ WHILE b DO c END ]=> st'), Q st') ->
+    exists st' (exe : Sigma |- st =[ WHILE b DO c END ]=> st'),
+      Q st' /\
+      (forall st'' (exe' : Sigma |- st =[ WHILE b DO c END ]=> st''),
+          Q st'' -> loop_size exe <= loop_size exe').
+  Proof.
+    intros.
+    edestruct (nonempty_smallest_ex
+                 (fun m => exists st' (exe : Sigma |- st =[ WHILE b DO c END ]=> st'),
+                      Q st' /\ loop_size exe = m)).
+    - firstorder eauto.
+    - destruct_conjs. subst. repeat econstructor; eauto.
+      Grab Existential Variables.
+      auto.
+  Qed. *)
+
+  Lemma ewp'_is_precondition {Sigma : Env}: forall c Q,
+      forall st,
+        ewp' Sigma c Q st ->
+        Productive Sigma c st Q.
+  Proof.
+    firstorder.
+  Qed.
+
+  Lemma ewp'_is_weakest (Sigma : Env) : forall c Q (P : Assertion),
+      (forall st, P st -> Productive Sigma c st Q) ->
+      P ->> ewp' Sigma c Q.
+  Proof.
+    firstorder.
+  Qed.
+
+  (* The Productive predicate and the existential hoare rules should
+  be equivalent. This proof will let us prove the soundness of vc
+  generation with respect to the hoare rules. *)
+  Theorem produces_ehoare_proof {Sigma : Env}
+    : forall c (P Q : Assertion),
+      productive_Env Sigma ->
+      (forall st,
+        P st ->
+        Productive {| funSigs := @funSigs Sigma;
+                      funSpecs := @funSpecs Sigma;
+                      funDefs := empty |} c st Q) ->
+        funSpecs |- {[P]} c {[Q]}#.
+  Proof.
+    induction c; intros.
+    - eapply EH_Consequence; eauto with hoare; intros.
+      eapply H0 in H1; remember CSkip in H1; clear H0.
+      induction H1; try congruence; injections.
+      + econstructor.
+      + eapply H0; apply IHProductive; eauto.
+    - eapply EH_Consequence; eauto with hoare; intros.
+      eapply H0 in H1; remember (CAss x a) in H1; clear H0.
+      induction H1; try congruence; injections.
+      + econstructor.
+      + eapply H0; apply IHProductive; eauto.
+    - eapply EH_Consequence; eauto with hoare; intros.
+      eapply H0 in H1; remember (CCall x f args) in H1; clear H0.
+      induction H1; try congruence; injections.
+      + simpl in H0; discriminate.
+      + firstorder eauto.
+      + firstorder eauto.
+    - apply EH_Seq with (fun st => Productive {| funSigs := funSigs; funSpecs := funSpecs; funDefs := empty |} c2 st Q); eauto.
+      + apply IHc1; eauto.
+        intros.
+        eapply H0 in H1; remember (CSeq c1 c2) in H1; clear H0.
+        induction H1; try congruence; injections.
+        * eapply Productive_Weaken; eauto with hoare; intros.
+        * eapply Productive_Weaken; eauto with hoare; intros.
+          unfold Included, In; intros; eauto using Productive_Weaken.
+    - apply EH_If.
+      + apply IHc1; intuition eauto.
+        eapply H0 in H2; remember (CIf b c1 c2) in H2; clear H0.
+        induction H2; try congruence; injections.
+        eapply Productive_Weaken; eauto with hoare; intros.
+      + apply IHc2; intuition eauto.
+        eapply H0 in H2; remember (CIf b c1 c2) in H2; clear H0.
+        induction H2; try congruence; injections.
+        eapply Productive_Weaken; eauto with hoare; intros.
+    - eapply EH_Consequence with (P' := fun st => ewp' {| funSigs := funSigs; funSpecs := funSpecs; funDefs := empty |} (WHILE b DO c END) Q st /\ (exists n : nat, loop_measureR' {| funSigs := funSigs; funSpecs := funSpecs; funDefs := empty |} b c Q n st)).
+      + eapply EH_While.
+        * intros; eapply IHc; eauto; intros st [Hwp [Hb Hm]].
+          unfold loop_measureR', ewp' in *.
+          remember (CWhile b c) in Hwp.
+          clear H0.
+          induction Hwp; try congruence; injections.
+          Focus 2.
+          (*eapply Productive_Weaken.
+          eapply IHHwp; eauto.
+          intros.
+          simpl in *.
+          Set Printing Implicit.
+          eapply Hm; eapply H0; eauto.
+          unfold Included, In; intros; intuition eauto using Productive_Weaken.
+          destruct H3 as [? [? ?] ]; eexists; intuition eauto.
+          eapply H1. *)  
+
+
+          admit.
+          admit.
+      + intros; eapply H0 in H1.
+        unfold ewp'; split; eauto.
+        unfold loop_measureR'.
+        eapply ewp'_loop_measureR'; eauto.
+      + simpl; intros st [? ?].
+        remember (CWhile b c) in H1; clear H0.
+        induction H1; try congruence; injections.
+        * econstructor.
+        * eapply H0; apply IHProductive; eauto.
+  Admitted.
 
 End EHoare.
 
